\documentclass{letter}
\usepackage{hyperref}
\usepackage{amsmath}
\usepackage{amsthm}
\signature{Ricardo Bittencourt}
\DeclareMathOperator{\csch}{csch}
\begin{document}

\newtheorem{lemma}{Lemma}

\begin{letter}{}
  \textbf{12338.} Prove:
  $$\int_0^\infty\frac{\cos\left(x\right)-1}{x\left(e^x-1\right)}\;dx
    = \frac{1}{2}\ln\left(\pi\csch\left(\pi\right)\right)$$

  \textbf{Solution.} We start with the series for $\cos x$:

\begin{align*}
  \int_0^\infty\frac{\cos\left(x\right)-1}{x\left(e^x-1\right)}\;dx
    &= \int_0^\infty\frac{\left(\sum_{n=0}^\infty\frac{(-1)^n x^{2n}}{(2n)!}
    \right)-1}{x\left(e^x-1\right)}\;dx \\
    &= \int_0^\infty\sum_{n=1}^\infty
      \frac{(-1)^n x^{2n-1}}{(2n)!\left(e^x-1\right)}\;dx \\
    &= \sum_{n=1}^\infty\frac{(-1)^n}{(2n)!}\int_0^\infty
      \frac{x^{2n-1}}{e^x-1}\;dx 
\end{align*}

We know the Riemann zeta can be expressed as an integral:

$$\zeta(s)=\frac{1}{\Gamma(s)}\int_0^\infty\frac{x^{s-1}}{e^x-1}\;dx$$

and therefore our previous integral can be expressed as $\zeta(2n)\Gamma(2n)$:

\begin{align*}
  \sum_{n=1}^\infty\frac{(-1)^n}{(2n)!}\int_0^\infty
      \frac{x^{2n-1}}{e^x-1}\;dx 
  &= \sum_{n=1}^\infty\frac{(-1)^n\zeta(2n)\Gamma(2n)}{(2n)!}\\
  &= \sum_{n=1}^\infty\frac{(-1)^n\zeta(2n)(2n-1)!}{(2n)!}\\
  &= \sum_{n=1}^\infty\frac{(-1)^n\zeta(2n)}{2n}
\end{align*}

The zeta function $\zeta(2n)$ can be expressed in closed form as a function of the Bernoulli numbers:

$$\zeta(2n)=\frac{(-1)^{n+1}B_{2n}(2\pi)^{2n}}{2(2n)!}$$

leading to:

\begin{align*}
  \sum_{n=1}^\infty\frac{(-1)^n\zeta(2n)}{2n} &= 
    \sum_{n=1}^\infty\frac{(-1)^n(-1)^{n+1}B_{2n}(2\pi)^{2n}}{4n(2n)!} \\
  &= \sum_{n=1}^\infty-\frac{B_{2n}(2\pi)^{2n}}{4n(2n)!}
\end{align*}

This last series we will solve with a lemma:

\begin{lemma}
$\ln(k \csch k) = 
   -\sum_{n=1}^\infty\frac{B_{2n}(2k)^{2n}}{2n(2n)!}$
\end{lemma}
\begin{proof}
We start with the logaritmic differentiation of $x \csch x$:

\begin{align*}
  \frac{d}{dx}\ln(x \csch x) &=
    \frac{1}{x \csch x}\left(\csch(x)- x\coth(x)\csch(x)\right)\\
    &= \frac{1}{x}-\coth(x)\\
\end{align*}

Using the series of $\coth x$:

$$\coth x=\sum_{n=0}^\infty\frac{2^{2n}B_{2n}x^{2n-1}}{(2n)!}$$

we have:

\begin{align*}
  \frac{1}{x}-\coth(x) &= \frac{1}{x} - 
    \sum_{n=0}^\infty\frac{2^{2n}B_{2n}x^{2n-1}}{(2n)!}\\
  &= -\sum_{n=1}^\infty\frac{2^{2n}B_{2n}x^{2n-1}}{(2n)!}
\end{align*}

At this point we can integrate both sides:

\begin{align*}
  \int_0^k\frac{d}{dx}\ln(x \csch x)\;dx 
    &= -\int_0^k\sum_{n=1}^\infty\frac{2^{2n}B_{2n}x^{2n-1}}{(2n)!}\;dx\\
  \ln(k \csch k) - \lim_{x\to 0}\ln(x \csch x) 
    &= -\sum_{n=1}^\infty\frac{2^{2n}B_{2n}}{(2n)!}\int_0^k x^{2n-1}\;dx\\
    &= -\sum_{n=1}^\infty\frac{2^{2n}B_{2n}}{(2n)!}
      \left(\frac{k^{2n}}{2n}\right)\\
    &= -\sum_{n=1}^\infty\frac{B_{2n}(2k)^{2n}}{2n(2n)!}
\end{align*}

The limit on the left side can be proven to be zero:
\begin{align*}
  \lim_{x\to 0}\ln(x \csch x) &=
    \ln\left(\lim_{x\to 0}x \csch x\right) \\
  &= \ln\left(\lim_{x\to 0}\frac{x}{\sinh x}\right) \\
  &= \ln\left(\lim_{x\to 0}\frac{1}{\cosh x}\right) \\
  &= 0
\end{align*}

This completes the proof.

\end{proof}

We finish the original integral by considering the series for $\ln(\pi \csch \pi)$:

\begin{align*}
  \int_0^\infty\frac{\cos\left(x\right)-1}{x\left(e^x-1\right)}
  &= \sum_{n=1}^\infty-\frac{B_{2n}(2\pi)^{2n}}{4n(2n)!} \\
  &= \frac{1}{2}\left(-\sum_{n=1}^\infty\frac{B_{2n}(2\pi)^{2n}}{2n(2n)!} 
  \right)\\
  &= \frac{1}{2}\ln(\pi \csch \pi)
\end{align*}



\end{letter}
\end{document}
