\documentclass{letter}
\usepackage{hyperref}
\usepackage{amsmath}
\usepackage{amsthm}
\signature{Ricardo Bittencourt}
\DeclareMathOperator{\csch}{csch}
\begin{document}

\newtheorem{lemma}{Lemma}

\begin{letter}{}
  \textbf{12398.} Evaluate:

  $$\sum_{n=0}^\infty \csch \left(2^n\right)$$.

  \textbf{Solution.} First we notice that $\coth(x/2)-\coth(x)=\csch(x)$. Using the definitions:

\begin{align*}
  \coth\left(x/2\right) - \coth\left(x\right) &=
  \frac{\mathrm{e}^x+1}{\mathrm{e}^x-1} 
  - \frac{\mathrm{e}^{2x}+1}{\mathrm{e}^{2x}-1}\\
  &=
  \frac{\mathrm{e}^x+1}{\mathrm{e}^x-1} 
  - \frac{\mathrm{e}^{2x}+1}{\left(\mathrm{e}^{x}-1\right)\left(\mathrm{e}^{x}-1\right)}\\
  &=
  \frac{\left(\mathrm{e}^x+1\right)^2 - \mathrm{e}^{2x} - 1}
  {\left(\mathrm{e}^{x}-1\right)\left(\mathrm{e}^{x}-1\right)}\\
  &=
  \frac{2\mathrm{e}^{x}}{\mathrm{e}^{2x}-1}\\
  &= \csch\left(x\right)
\end{align*}

Now the original sum telescopes:

\begin{align*}
  \sum_{n=0}^\infty \csch \left(2^n\right)
  &=
  \lim_{t\to \infty} 
  \sum_{n=0}^t
    \coth \left(2^{n-1}\right) - \coth \left(2^n\right)\\
  &= 
    \lim_{t\to \infty} 
    \coth \left(1/2\right) + 
        \sum_{n=1}^t \coth\left(2^{n-1}\right) - 
        \sum_{n=0}^{t-1} \coth\left(2^{n}\right)
    - \coth\left(2^t\right)\\
  &= 
    \lim_{t\to \infty} 
    \coth \left(1/2\right)  
    - \coth\left(2^t\right)\\
  &= \coth\left(1/2\right) - 1
\end{align*}

Plugging in the definition we have our closed form: 

$$\sum_{n=0}^\infty \csch \left(2^n\right)
  = \coth\left(1/2\right) - 1 = \frac{\mathrm{e}+1}{\mathrm{e}-1}-1
  = \frac{2}{\mathrm{e}-1}$$

\end{letter}
\end{document}
