\documentclass{letter}
\usepackage{hyperref}
\usepackage{amsmath}
\usepackage{amsthm}
\signature{Ricardo Bittencourt}
\DeclareMathOperator{\csch}{csch}
\begin{document}

\newtheorem{lemma}{Lemma}

\begin{letter}{}
  \textbf{12344.} An integer is a \textit{one-drop number} if its decimal digits $d_1\ldots d_n$ satisfy $1\le d_1 \le \ldots\le d_i > d_{i+1} \le \ldots\le d_n$ for some $i$. For example, $13802$ and $49557$ are one-drop numbers. For $n \ge 2$, how many $n$-digit one-drop numbers are there?

  \textbf{Solution.} We'll use the analytic combinatorics from Flajolet and Sedgewick. Let $SEQ(z)$ be the set of sequences of the digit $z$, and $SEQ_{\ge 1}(z)$ be the set of non-empty sequences of $z$. Their generating functions are given by:

\begin{align*}
SEQ(z) &= \frac{1}{1-z} \\
SEQ_{\ge 1}(z) &= \frac{1}{1-z} - 1 = \frac{z}{1-z} 
\end{align*} 

Suppose the digits where the drop occur are $a$ and $b$, with $b<a$. The generating function of the one-drop numbers with these digits in the drop are:

$$F(a, b) = SEQ(1)\ldots SEQ(a-1)SEQ_{\ge 1}(a)SEQ_{\ge 1}(b)SEQ(b+1)\ldots SEQ(9)$$

The generating function of all one-drop numbers is, therefore, the sum of the previous generating functions for all valid $a, b$:

\begin{align*}
G(z) &= \sum_{1\le a\le 9}\,\sum_{0 \le b < a} F(a,b) \\
     &= \sum_{1\le a\le 9}\,\sum_{0 \le b < a} SEQ(z)^{a-1}\, SEQ_{\ge 1}(z)\, SEQ_{\ge 1}(z)\, SEQ(z)^{9-b}\\
     &= \sum_{1\le a\le 9}\,\sum_{0 \le b < a} SEQ(z)^{8+a-b}\,SEQ_{\ge 1}(z)^2\\
     &= \sum_{1\le a\le 9}\,\sum_{0 \le b < a} \left(\frac{1}{1-z}\right)^{8+a-b}\,\left(\frac{z}{1-z}\right)^2\\
     &=  \frac{z^2}{(1-z)^{10}}\sum_{1\le a\le 9}\,\left(\frac{1}{1-z}\right)^{a}
\sum_{0 \le b < a} \left(1-z\right)^{b}\\
     &=  \frac{z^2}{(1-z)^{10}}\sum_{1\le a\le 9}\,\left(\frac{1}{1-z}\right)^{a}\left(\frac{1-\left(1-z\right)^{a}}{z}\right)\\
     &=  \frac{z}{(1-z)^{10}}\left(\sum_{1\le a\le 9}\,\left(\frac{1}{1-z}\right)^{a}-\sum_{1\le a\le 9}\,1\right)\\
     &=  \frac{1}{(1-z)^{10}}\left(\frac{1-\left(1-z\right)^9}{\left(1-z\right)^9}-9z\right)\\
     &=  \frac{1}{(1-z)^{19}}-\frac{1}{(1-z)^{10}}-\frac{9z}{(1-z)^{10}}
\end{align*}

The coefficients can be extracted directly, since $1/(1-z)^{k+1} = \sum_{n\ge 0}{n+k\choose k}x^n$ and multiplying by $z$ is a shift in the coefficients. The solution to the problem is:

\begin{align*}
[z^n]G(z) &= {n+18\choose 18}-{n+9\choose 9}-9{n+8\choose 9}
\end{align*}

\end{letter}
\end{document}
