\documentclass{letter}
\usepackage{hyperref}
\usepackage{amsmath}
\usepackage{amsthm}
\signature{Ricardo Bittencourt}
\DeclareMathOperator{\csch}{csch}
\begin{document}

\newtheorem{lemma}{Lemma}

\begin{letter}{}

  \textbf{2161.} Let $x_n$ denote the number of bitstrings of length $n$ which contain neither $11$ nor $000$ as substrings. Find a recursive formula for $x_n$.

  \textbf{Solution.}

  The desired bitstrings match the following regular expression, where $?$ denote an optional expression, $|$ is the exclusive or operator, and $*$ is the Kleene star:

$$1?((0|00)1)*(0|00)?$$

  Using Flajolet's Analytic Combinatorics, this regular expression can be directly converted into a generating funcion, by replacing concatenation with multiplication, exclusive or with addition, optional expressions with $(1+f(z))$ and the Kleene star with $1/(1-f(z))$.

  $$X(z)=\left(1 + z\right)\frac{1}{1-\left(z+z^2\right)z}\left(1+z+z^2\right)
  =\frac{(1+z)(1+z+z^2)}{1-z^2-z^3}$$

The desired recursive formula can be extracted directly from the definition of the generating function:

  \begin{align*}
  X(z) &= \frac{(1+z)(1+z+z^2)}{1-z^2-z^3} \\
  \left(1-z^2-z^3\right)\sum_{n\ge 0}x_n z^n &= (1+z)(1+z+z^2) \\
  \sum_{n\ge 0}x_n z^n - \sum_{n\ge 0}x_n z^{n+2} - \sum_{n\ge 0}x_n z^{n+3} 
  &= 1+2z+2z^2+z^3\\
  \sum_{n\ge 0}x_n z^n - \sum_{n\ge 2}x_{n-2} z^n - \sum_{n\ge 3}x_{n-3} z^n 
  &= 1+2z+2z^2+z^3
  \end{align*}

The general recurrence can be extracted from the coefficients above when $n\ge 4$:

  \begin{align*}
  [z^n]\left(\sum_{n\ge 0}x_n z^n - \sum_{n\ge 2}x_{n-2} z^n - \sum_{n\ge 3}x_{n-3} z^n \right)
  &= [z^n]\left(1+2z+2z^2+z^3\right)\\
  x_n - x_{n-2} - x_{n-3}  &= 0\\
  x_n &= x_{n-2} + x_{n-3}
  \end{align*}

The initial conditions can be read when $n$ is small. Since the order of the recurrence is 3, we need 3 initial values:

\begin{align*}
n = 0 &\implies x_0 = 1 \\
n = 1 &\implies x_1 = 2 \\
n = 2 &\implies x_2 - x_0 = 2 \implies x_2 = 3\\
\end{align*}

Therefore, the final recurrence formula is:

$$x_n=\begin{cases}
  n+1 & \text{if $n < 3$} \\
  x_{n-2}+x_{n-3} & \text{if $n \ge 3$}
  \end{cases}$$


\end{letter}
\end{document}
