\documentclass{letter}
\usepackage{hyperref}
\usepackage{amsmath}
\usepackage{amsthm}
\signature{Ricardo Bittencourt}
\DeclareMathOperator{\csch}{csch}
\begin{document}

\newtheorem{lemma}{Lemma}
\newcommand\term[1]{\frac{x^{#1}}{#1!}}

\begin{letter}{}

  \textbf{2171.} Evaluate the following sums in closed form.

  (a) $\displaystyle{\sum_{n=0}^{\infty}\left(\cos x -1 +\term{2}-\term{4}+\cdots+
    \left(-1\right)^{n-1}\frac{x^{2n}}{\left(2n\right)!}   \right)}$

  (b) $\displaystyle{\sum_{n=0}^{\infty}\left(\sin x -x +\term{3}-\term{5}+\cdots+
    \left(-1\right)^{n-1}\frac{x^{2n+1}}{\left(2n+1\right)!}   \right)}$
  
  \textbf{Solution.}

  For the item (a), we start by writing the infinite sum in a more concise format, and then open the $\cos$ in a series:

  \begin{align*}
  A(x) &= \sum_{n=0}^{\infty}\left(\cos x -1 +\term{2}-\term{4}+\cdots+
    \left(-1\right)^{n-1}\frac{x^{2n}}{\left(2n\right)!}   \right) \\
       &= \sum_{n=0}^{\infty}\left(\cos x 
    -\sum_{k=0}^{n}\left(-1\right)^k \frac{x^{2k}}{(2k)!} \right)\\
       &= \sum_{n=0}^{\infty}\left(
    \sum_{k=0}^{\infty}\left(-1\right)^k \frac{x^{2k}}{(2k)!} 
    -\sum_{k=0}^{n}\left(-1\right)^k \frac{x^{2k}}{(2k)!} \right) \\
       &= \sum_{n=0}^{\infty}\left(
    \sum_{k=n+1}^{\infty}\left(-1\right)^k \frac{x^{2k}}{(2k)!} \right)\\
       &= \sum_{k\ge 1}\left(
    \sum_{0\le n < k}\left(-1\right)^k \frac{x^{2k}}{(2k)!} \right)\\
       &= \sum_{k\ge 1}\left(k
    \left(-1\right)^k \frac{x^{2k}}{(2k)!} \right)\\
  \end{align*}

  At this point we can multiply by $2/x$ and introduce $q=k-1$ to get the result:
  \begin{align*}
  A(x) &= \sum_{k\ge 1}\left(k\left(-1\right)^k \frac{x^{2k}}{(2k)!} \right) \\
  \frac{2}{x}A(x) &= \sum_{k\ge 1}\left(2k\left(-1\right)^k \frac{x^{2k-1}}{(2k)!} \right) \\
    &= \sum_{k\ge 1}\left(\left(-1\right)^k \frac{x^{2k-1}}{(2k-1)!} \right) \\
    &= \sum_{k\ge 1}\left(-1\right)^k \frac{x^{2k-1}}{(2k-1)!} \\
    &= \sum_{q\ge 0}\left(-1\right)^{q+1} \frac{x^{2q+1}}{(2q+1)!} \\
    &= -\sin x \\
  A(x) &= -\frac{x\sin x}{2}\\
  \end{align*}
  
  The calculations for item (b) are similar:

  \begin{align*}
  B(x) &= \sum_{n=0}^{\infty}\left(\sin x -x +\term{3}-\term{5}+\cdots+
    \left(-1\right)^{n-1}\frac{x^{2n+1}}{\left(2n+1\right)!}   \right) \\
       &= \sum_{n=0}^{\infty}\left(
    \sum_{k=0}^{\infty}\left(-1\right)^k \frac{x^{2k+1}}{(2k+1)!} 
    -\sum_{k=0}^{n}\left(-1\right)^k \frac{x^{2k+1}}{(2k+1)!} \right) \\
       &= \sum_{n=0}^{\infty}\left(
    \sum_{k=n+1}^{\infty}\left(-1\right)^k \frac{x^{2k+1}}{(2k+1)!} \right)\\
       &= \sum_{k\ge 1}\left(
    \sum_{0\le n < k}\left(-1\right)^k \frac{x^{2k+1}}{(2k+1)!} \right)\\
       &= \sum_{k\ge 1}\left(k
    \left(-1\right)^k \frac{x^{2k+1}}{(2k+1)!} \right)\\
  \end{align*}

  This time we multiply by $2$ and split the sum into two parts:
  
  \begin{align*}
    B(x) &= \sum_{k\ge 1}\left(k
    \left(-1\right)^k \frac{x^{2k+1}}{(2k+1)!} \right)\\
    2B(x) &= \sum_{k\ge 1}\left(2k
    \left(-1\right)^k \frac{x^{2k+1}}{(2k+1)!} \right)\\
    &= \sum_{k\ge 1}\left((2k+1-1)
    \left(-1\right)^k \frac{x^{2k+1}}{(2k+1)!} \right)\\
    &= \sum_{k\ge 1}\left(\left(-1\right)^k \frac{x^{2k+1}}{(2k)!} \right)
      - \sum_{k\ge 1}\left(\left(-1\right)^k \frac{x^{2k+1}}{(2k+1)!} \right) \\
    &= x\sum_{k\ge 1}\left(\left(-1\right)^k \frac{x^{2k}}{(2k)!} \right)
      - (\sin x - x) \\
    &= x(\cos x - 1) - (\sin x - x) \\
    &= x\cos x - \sin x \\
    B(x) &= \frac{x\cos x - \sin x}{2}
  \end{align*}

\end{letter}
\end{document}
