\documentclass{letter}
\usepackage{hyperref}
\usepackage{amsmath}
\usepackage{amsthm}
\signature{Ricardo Bittencourt}
\begin{document}

\newtheorem{lemma}{Lemma}

\begin{letter}{}

  \textbf{2147.} Evaluate:
  $$\prod_{n=2}^{\infty}\frac{n^4+4}{n^4-1}$$

  \textbf{Solution.} We start by factoring and completing squares:

\begin{align*}
\prod_{n=2}^{\infty}\frac{n^4+4}{n^4-1} &=
  \prod_{n=2}^{\infty}\frac{n^4+4n^2+4-4n^2}
  {\left(n^2+1\right)\left(n^2-1\right)} \\
  &= \prod_{n=2}^{\infty}\frac{\left(n^2+2\right)^2-\left(2n\right)^2}
  {\left(n^2+1\right)\left(n+1\right)\left(n-1\right)} \\
  &= \prod_{n=2}^{\infty}\frac{\left(n^2+2n+2\right)\left(n^2-2n+2\right)}
  {\left(n^2+1\right)\left(n+1\right)\left(n-1\right)} \\
  &= \prod_{n=2}^{\infty}\frac{\left(n^2+2n+1+1\right)\left(n^2-2n+1+1\right)}
  {\left(n^2+1\right)\left(n+1\right)\left(n-1\right)} \\
  &= \prod_{n=2}^{\infty}\frac{\left(\left(n+1\right)^2+1\right)
  \left(\left(n-1\right)^2+1\right)}
  {\left(n^2+1\right)\left(n+1\right)\left(n-1\right)} \\
\end{align*}

At this point we can split the expression into five products, and change their indexes:
$$  \prod_{n=2}^{\infty}\frac{\left(\left(n+1\right)^2+1\right)
  \left(\left(n-1\right)^2+1\right)}
  {\left(n^2+1\right)\left(n+1\right)\left(n-1\right)} = A B C D E $$

\begin{align*}
  A &= \prod_{n=2}^{\infty}\left(n+1\right)^2+1
     = \prod_{n=3}^{\infty}n^2+1
     = \frac{1}{\left(1^2+1\right)\left(2^2+1\right)}
       \prod_{n=1}^{\infty}n^2+1 
     = \frac{1}{10} \prod_{n=1}^{\infty}n^2+1 \\
  B &= \prod_{n=2}^{\infty}\left(n-1\right)^2+1
     = \prod_{n=1}^{\infty}n^2+1 \\
  C &= \prod_{n=2}^{\infty}\frac{1}{n^2+1} 
     = \left(1^2+1\right)\prod_{n=1}^{\infty}\frac{1}{n^2+1}
     = 2\prod_{n=1}^{\infty}\frac{1}{n^2+1} \\
  D &= \prod_{n=2}^{\infty}\frac{1}{n+1} 
     = \prod_{n=3}^{\infty}\frac{1}{n} 
     = \left(1\right)\left(2\right)\prod_{n=1}^{\infty}\frac{1}{n} 
     = 2\prod_{n=1}^{\infty}\frac{1}{n} \\
  E &= \prod_{n=2}^{\infty}\frac{1}{n-1} 
     = \prod_{n=1}^{\infty}\frac{1}{n} 
\end{align*}

Joining the products again, we obtain:

\begin{align*}
ABCDE &= 
     \frac{2}{5} \prod_{n=1}^{\infty}
     \frac{\left(n^2+1\right) \left(n^2+1\right)}
     {\left(n^2+1\right)\left(n\right)\left(n\right)} \\
  &= \frac{2}{5} \prod_{n=1}^{\infty}
     \frac{n^2+1}{n^2}\\
  &= \frac{2}{5} \prod_{n=1}^{\infty}
     1+\frac{1}{n^2}
\end{align*}

This expression can be simplified with the well-known formula for $\sinh$:

\begin{align*}
  \sinh\left(x\right) &=
  x \prod_{n=1}^{\infty}1+\frac{x^2}{n^2 \pi^2} \\
  \sinh\left(\pi x\right) &= \pi x
    \prod_{n=1}^{\infty}1+\frac{\left(\pi x\right)^2}{n^2 \pi^2} \\
  \frac{\sinh\left(\pi x\right)}{\pi x} &= 
    \prod_{n=1}^{\infty}1+\frac{x^2}{n^2}
\end{align*}

By using $x=1$, we arrive at the final expression:

\begin{align*}
  \frac{2}{5} \prod_{n=1}^{\infty}
     1+\frac{1}{n^2} &= 
  \frac{2}{5} \left(\frac{\sinh\left(\pi\right)}{\pi}\right) \\
  &= \frac{2\sinh\left(\pi\right)}{5\pi} 
\end{align*}

\end{letter}
\end{document}
