\documentclass{letter}
\usepackage{hyperref}
\usepackage{amsmath}
\usepackage{amsthm}
\signature{Ricardo Bittencourt}
\DeclareMathOperator{\csch}{csch}
\DeclareMathOperator\arctanh{arctanh}
\begin{document}

\newtheorem{lemma}{Lemma}
\newcommand\term[1]{\frac{x^{#1}}{#1!}}

\begin{letter}{}
  \textbf{2186.} Evaluate

  $$\int_0^1\frac{\arctanh\left(x \sqrt{2-x^2}\right)}{x}\;dx $$

 
  \textbf{Solution.}

  Let $x=\sqrt{1-\cos\theta}$. It follows that $x\sqrt{2-x^2}=\sin\theta$ and the integral becomes:

  \begin{align*}
  \int_0^1\frac{\arctanh\left(x \sqrt{2-x^2}\right)}{x}\;dx 
    &=
    \int_0^{\pi/2}\frac
      {\arctanh\left(\sin\theta
      \right)}
    {\sqrt{1-\cos\theta}}\left(\frac{\sin\theta}{2\sqrt{1-\cos\theta}}\right)\;d\theta\\
    &=
    \frac{1}{2}\int_0^{\pi/2}\frac
      {\sin\theta\arctanh\left(\sin\theta\right)}
    {1-\cos\theta}\;d\theta\\
    &=
    \frac{1}{2}\int_0^{\pi/2}\frac
      {\sin\theta\arctanh\left(\sin\theta\right)}
    {1-\cos\theta}\left(\frac
    {1+\cos\theta}{1+\cos\theta}\right)\;d\theta\\
    &=
    \frac{1}{2}\int_0^{\pi/2}\frac
      {\sin\theta(1+\cos\theta)\arctanh\left(\sin\theta\right)}
    {(\sin\theta)^2}\;d\theta\\
    &=
    \frac{1}{2}\int_0^{\pi/2}\frac
      {(1+\cos\theta)\arctanh\left(\sin\theta\right)}
    {\sin\theta}\;d\theta\\
    &=
    \frac{1}{2}\int_0^{\pi/2}\frac
      {\arctanh\left(\sin\theta\right)}
    {\sin\theta}\;d\theta
    +\frac{1}{2}\int_0^{\pi/2}\frac
      {\cos\theta\arctanh\left(\sin\theta\right)}
    {\sin\theta}\;d\theta
    \\
  \end{align*}

  For the first integral, let's introduce a parameter $a$ and then differentiate it:

  \begin{align*}
    I(a) &=
    \int_0^{\pi/2}\frac
      {\arctanh\left(a \sin\theta\right)}
    {\sin\theta}\;d\theta\\
    I'(a) &= \frac{d}{da}
      \int_0^{\pi/2}\frac
        {\arctanh\left(a \sin\theta\right)}
      {\sin\theta}\;d\theta\\
      &=
      \int_0^{\pi/2}\frac{\partial}{\partial a}\frac
        {\arctanh\left(a \sin\theta\right)}
      {\sin\theta}\;d\theta\\
      &=
      \int_0^{\pi/2}\left(\frac{\sin\theta}{1-a^2\sin^2\theta}\right)
      \frac{1}{\sin\theta}\;d\theta\\
      &=
      \int_0^{\pi/2}\frac{1}{1-a^2\sin^2\theta}\;d\theta
  \end{align*}

  With the substitution $u=\cot\theta$, followed by $s=\frac{u}{\sqrt{1-a^2}}$, we have:

  \begin{align*}
    I'(a) &= 
      \int_{\infty}^0\frac{1}{1-a^2\frac{1}{1+u^2}}\left(\frac{1}{-1-u^2}\right)\;du\\
      &= \int_{\infty}^{0}\frac{1}{a^2-1-u^2}\;du\\
      &= \frac{1}{1-a^2}\int_0^\infty\frac{1}{1+\frac{u^2}{1-a^2}}\;du\\
      &= \frac{1}{1-a^2}\int_0^\infty\frac{1}{1+s^2}\left(\sqrt{1-a^2}\right)\;ds\\
      &= \frac{1}{\sqrt{1-a^2}}\left(\arctan s\right)_0^\infty\\
      &= \frac{\pi}{2}\frac{1}{\sqrt{1-a^2}}\\
    I(a) &= \frac{\pi}{2}\arcsin a + C
  \end{align*}

  By setting $a=0$, it's clear that $I(0)=0$, and therefore $C=0$. The first integral can be evaluated by setting $a=1$:

  $$I(1)=\frac{\pi}{2}\arcsin 1=\frac{\pi^2}{4}$$

  For the second integral we again introduce a parameter $a$:

  \begin{align*}
    J(a) &=
    \int_0^{\pi/2}\frac
      {\cos\theta\arctanh\left(a \sin\theta\right)}
    {\sin\theta}\;d\theta\\
    J'(a) &= 
      \int_0^{\pi/2}\frac
        {\cos\theta}{\sin\theta}\left(\frac{\sin\theta}{1-a^2\sin^2\theta}\right)\;d\theta\\
        &=
      \int_0^{\pi/2}\frac
        {\cos\theta}{1-a^2\sin^2\theta}\;d\theta
  \end{align*}

  The substitution $u=a\sin\theta$ leads to:

  \begin{align*}
    J'(a) &=\frac{1}{a}\int_0^a\frac{1}{1-u^2}\;du\\
    &=\frac{1}{a}\left(\arctanh u\right)_0^a \\
    &=\frac{\arctanh a}{a}\\
    J(a)&=\int\frac{\arctanh a}{a}\;da
  \end{align*}

  Replacing $\arctanh$ with its Taylor series we get:

  \begin{align*}
    J(a) &= \int\frac{1}{a}\sum_{n\ge 1}\frac{a^{2n-1}}{2n-1} \\
    &=\sum_{n\ge 1}\int\frac{a^{2n-2}}{2n-1}\;da \\
    &=\sum_{n\ge 1}\left(\frac{a^{2n-1}}{(2n-1)^2}+C\right) \\
  \end{align*}

  For $a=0$ we should again have $J(0)=0$, which implies $C=0$. The desired value for the second integral is $J(1)$:

  \begin{align*}
    J(1) &= \sum_{n\ge 1}\frac{1}{(2n-1)^2}\\
    &= \sum_{n\ge 1}\frac{1}{n^2}-\sum_{n\ge 1}\frac{1}{(2n)^2}\\
    &= \sum_{n\ge 1}\frac{1}{n^2}-\frac{1}{4}\sum_{n\ge 1}\frac{1}{n^2}\\
    &= \left(1-\frac{1}{4}\right)\zeta(2)\\
    &=\frac{3}{4}\left(\frac{\pi^2}{6}\right)\\
    &=\frac{\pi^2}{8}
  \end{align*}

  The original integral now can be determined by our previous results:

  \begin{align*}
  \int_0^1\frac{\arctanh\left(x \sqrt{2-x^2}\right)}{x}\;dx 
    &=\frac{1}{2}I(1)+\frac{1}{2}J(1)\\
    &=\frac{1}{2}\left(\frac{\pi^2}{4}+\frac{\pi^2}{8}\right)\\
    &=\frac{3\pi^2}{16}
  \end{align*}
  


\end{letter}
\end{document}
